examples/Yield/Lang.v
@@ -1,0 +1,139 @@
+From Coq Require Import
+     Arith.PeanoNat
+     Lists.List
+     Strings.String
+     Morphisms
+     Setoid
+     RelationClasses.
+
+From ExtLib Require Import
+     Data.String
+     Structures.Monad
+     Structures.Traversable
+     Data.List
+     Data.Map.FMapAList.
+
+From ITree Require Import
+     ITree
+     Basics.CategoryKleisli
+     Events.State
+     Events.StateFacts.
+
+From CTree Require Import
+     CTrees
+     Utils.
+
+From CTreeYield Require Import
+     Par.
+
+(* From ITree Require Import *)
+(*      ITree *)
+(*      ITreeFacts *)
+(*      Events.MapDefault *)
+(*      Events.StateFacts. *)
+
+(* Import Monads. *)
+Import MonadNotation.
+Local Open Scope monad_scope.
+Local Open Scope string_scope.
+
+(** Imp manipulates a countable set of variables represented as [string]s: *)
+Definition var : Set := string.
+
+(** For simplicity, the language manipulates [nat]s as values. *)
+Definition value : Type := nat.
+
+Inductive expr : Type :=
+| Var (_ : var)
+| Lit (_ : value)
+| Plus  (_ _ : expr)
+| Minus (_ _ : expr)
+| Mult  (_ _ : expr).
+
+Inductive stmt : Type :=
+| Assign (x : var) (e : expr)    (* x = e *)
+| Seq    (a b : stmt)            (* a ; b *)
+| If     (i : expr) (t e : stmt) (* if (i) then { t } else { e } *)
+| While  (t : expr) (b : stmt)   (* while (t) { b } *)
+| Spawn  (t : stmt)
+| Skip                           (* ; *)
+.
+
+Variant ImpState : Type -> Type :=
+| GetVar (x : var) : ImpState value
+| SetVar (x : var) (v : value) : ImpState unit.
+
+(* Inductive spawn1E (E : Type -> Type) : Type -> Type := *)
+(* | Spawn1 : forall (t : ctree (E +' spawn1E E) unit), spawn1E E unit. *)
+
+(* Inductive spawnE C (E : Type -> Type) : Type -> Type := *)
+(* | Spawn : forall (t: C -> ctree (E +' spawnE C E) (C * unit)), spawnE C E unit. *)
+
+Section Denote1.
+
+
+  (* Context {E' : Type -> Type}. *)
+  (* Context {HasImpState : ImpState -< E'}. *)
+  Definition E : Type -> Type := stateE value +' spawnE.
+  (* Context {HasSpawn1 : spawn1E  -< eff}. *)
+
+  Fixpoint denote_expr (e : expr) : ctree E value :=
+    match e with
+    | Var v     => trigger (Get _)
+    | Lit n     => ret n
+    | Plus a b  => l <- denote_expr a ;; r <- denote_expr b ;; ret (l + r)
+    | Minus a b => l <- denote_expr a ;; r <- denote_expr b ;; ret (l - r)
+    | Mult a b  => l <- denote_expr a ;; r <- denote_expr b ;; ret (l * r)
+    end.
+
+  Definition while (step : ctree E (unit + unit)) : ctree E unit :=
+    CTree.iter (fun _ => step) tt.
+
+  Definition is_true (v : value) : bool := if (v =? 0)%nat then false else true.
+
+  Fixpoint denote_imp (s : stmt) : ctree E unit :=
+    match s with
+    | Assign x e =>  v <- denote_expr e ;; trigger (Put _ v)
+    | Seq a b    =>  denote_imp a ;; denote_imp b
+    | If i t e   =>
+      v <- denote_expr i ;;
+      if is_true v then denote_imp t else denote_imp e
+
+    | While t b =>
+      while (v <- denote_expr t ;;
+	         if is_true v
+             then denote_imp b ;; ret (inl tt)
+             else ret (inr tt))
+
+    | Spawn t => vis Par.Spawn (fun b : bool =>
+                                 if b
+                                 then (denote_imp t;; ChoiceI 0 (fun _ => ret tt)) (* force the thread to halt here *)
+                                 else ret tt)
+    | Skip => ret tt
+    end.
+
+  Definition h_state {E} : forall X, stateE value X -> Monads.stateT value (ctree E) X :=
+    fun _ e s =>
+      match e with
+      | Get _ => Ret (s, s)
+      | Put _ s' => Ret (s', tt)
+      end.
+
+  #[global] Instance MonadChoice_stateT {M S} {MM : Monad M} {AM : Utils.MonadChoice M}
+    : Utils.MonadChoice (Monads.stateT S M).
+  Admitted.
+
+  Definition handler : forall X, E X -> Monads.stateT value (ctree spawnE) X :=
+    (fun X (e : E X) =>
+       match e with
+       | inl1 e' => @h_state spawnE _ e'
+       | inr1 e' =>
+         match e' in spawnE R return Monads.stateT value (ctree spawnE) R with
+         | Par.Spawn => fun s => b <- trigger Par.Spawn;; Ret(s, b) (* TODO: use MonadTrigger *)
+         end
+       end).
+
+  Definition interp_state (t : ctree E unit) : Monads.stateT value (ctree spawnE) unit :=
+    Interp.interp handler t.
+
+End Denote1.
